kremlib/Spec.Loops.fst
@@ -1,0 +1,34 @@
+module Spec.Loops
+
+#reset-options "--max_fuel 0"
+
+val seq_map:
+  #a:Type -> #b:Type ->
+  f:(a -> Tot b) ->
+  s:Seq.seq a ->
+  Tot (s':Seq.seq b{Seq.length s = Seq.length s' /\
+    (forall (i:nat). {:pattern (Seq.index s' i)} i < Seq.length s' ==> Seq.index s' i == f (Seq.index s i))})
+    (decreases (Seq.length s))
+let rec seq_map #a #b f s =
+  if Seq.length s = 0 then
+    Seq.createEmpty
+  else
+    let s' = Seq.cons (f (Seq.head s)) (seq_map f (Seq.tail s)) in
+    s'
+
+
+val seq_map2:
+  #a:Type -> #b:Type -> #c:Type ->
+  f:(a -> b -> Tot c) ->
+  s:Seq.seq a -> s':Seq.seq b{Seq.length s = Seq.length s'} ->
+  Tot (s'':Seq.seq c{Seq.length s = Seq.length s'' /\
+    (forall (i:nat). {:pattern (Seq.index s'' i)} i < Seq.length s'' ==> Seq.index s'' i == f (Seq.index s i) (Seq.index s' i))})
+    (decreases (Seq.length s))
+let rec seq_map2 #a #b #c f s s' =
+  if Seq.length s = 0 then Seq.createEmpty
+  else
+    let s'' = Seq.cons (f (Seq.head s) (Seq.head s')) (seq_map2 f (Seq.tail s) (Seq.tail s')) in
+    s''
+
+val repeat_spec: #a:Type -> n:nat -> (f: a -> Tot a) -> a -> Tot a (decreases n)
+let rec repeat_spec #a n f x = if n = 0 then x else repeat_spec (n-1) f (f x)
